HoareLogic/HoareLogic.v
@@ -6,14 +6,64 @@ Class HoareLogic (Imp: ImperativeProgrammingLanguage) (L: Language): Type := {
 }.
 
 Local Open Scope logic_base.
-
+(*
 Definition triple_valid {Imp: ImperativeProgrammingLanguage} {nImp: NormalImperativeProgrammingLanguage Imp} {L: Language} {MD: Model} {sss: SmallStepSemantics Imp MD} {SM: Semantics L MD} (guard: exceptional_state -> Prop) (Pre: expr) (c: cmd) (Post: expr): Prop :=
-  (forall (s_pre: state) (s_post: exceptional_state), access (inl (c, s_pre)) (inr s_post) -> s_pre |= Pre -> guard s_post) /\
-  (forall (s_pre: state) (s_post: state), access (inl (c, s_pre)) (inl (Sskip, s_post)) -> s_pre |= Pre -> s_post |= Post).
+  forall (s_pre: state) (ms_post: state + exceptional_state), access (inl s_pre) c ms_post -> s_pre |= Pre ->
+  match ms_post with
+  | inl s_post => s_post |= Post
+  | inr e => guard e
+  end.
 
 Section soundness.
 
-Context {Imp: ImperativeProgrammingLanguage} {nImp: NormalImperativeProgrammingLanguage Imp} {L: Language} {MD: Model} {sss: SmallStepSemantics Imp MD} {SM: Semantics L MD} (guard: exceptional_state -> Prop).
+Context {Imp: ImperativeProgrammingLanguage} {nImp: NormalImperativeProgrammingLanguage Imp} {MD: Model} {sss: SmallStepSemantics Imp MD}.
+
+Lemma exception_go_nowhere: forall e c ms,
+  access (inr e) c ms <->
+  ms = inr e.
+Proof.
+  intros.
+  split; intros.
+  + hnf in H.
+    remember (fmap_pair_cmd (inr e) c) as mcs1 eqn:?H.
+    remember (fmap_pair_cmd ms Sskip) as mcs2 eqn:?H.
+    induction H.
+    - subst.
+      destruct ms; inversion H1.
+      subst; auto.
+    - subst.
+      inversion H0.
+  + subst.
+    hnf.
+    simpl.
+    apply iter_step_refl.
+Qed.
+
+Lemma aux_sequence_sound: forall c1 c2 ms1 ms3,
+  access ms1 (Ssequence c1 c2) ms3 ->
+  exists ms2,
+  access ms1 c1 ms2 /\ access ms2 c2 ms3.
+Proof.
+  intros.
+  destruct ms1 as [s1 | e1].
+  Focus 2. {
+    exists (inr e1).
+    rewrite exception_go_nowhere in H.
+    subst.
+    split; rewrite exception_go_nowhere; auto.
+  } Unfocus.
+  unfold access in H.
+  remember (fmap_pair_cmd (inl s1) (Ssequence c1 c2)) as mcs1 eqn:?H.
+  remember (fmap_pair_cmd ms3 Sskip) as mcs2 eqn:?H.
+  revert c1 H0.
+  induction H; intros; subst.
+  + destruct ms3 as [s3 | e3]; inversion H0.
+    apply neq_Sskip_Ssequence in H1; contradiction.
+  + rename IHiter_step into IH.
+    specialize (IH eq_refl).
+    inversion H2; subst; clear H2.
+
+Context {L: Language} {SM: Semantics L MD} (guard: exceptional_state -> Prop).
 
 Lemma hoare_sequence_sound: forall c1 c2 P Q R,
   triple_valid guard P c1 Q ->
@@ -21,13 +71,18 @@ Lemma hoare_sequence_sound: forall c1 c2 P Q R,
   triple_valid guard P (Ssequence c1 c2) R.
 Proof.
   intros.
-  split; intros.
-  + remember (inl (Ssequence c1 c2, s_pre)) as mcs1 eqn:?H.
-    remember (inr s_post) as mcs2 eqn:?H.
-    revert c1 H H3.
-    induction H1; intros; subst.
-    - inversion H3.
-    - inversion H3; subst; clear H3.
+  hnf; intros.
+  unfold access in H1.
+  remember (fmap_pair_cmd (inl s_pre) (Ssequence c1 c2)) as mcs1 eqn:?H.
+  remember (fmap_pair_cmd ms_post Sskip) as mcs2 eqn:?H.
+  revert P c1 H H2 H3.
+  induction H1; intros; subst.
+  + destruct ms_post as [s_post | e]; [| inversion H3].
+    inversion H3; clear H3.
+    apply neq_Sskip_Ssequence in H4; contradiction.
+  + rename IHiter_step into IH.
+    specialize (IH eq_refl).
 Abort.
 
 End soundness.
+*)
